\documentclass{article}
\usepackage{amsmath}

\begin{document}
\begin{equation}
\begin{split}
3x_{3} = 9 \\
x_{1} + 5x_{2} - 2x_{3} = 2 \\
\frac{1}{3}x_{1} + 2x_{2} = 3
\end{split}
\end{equation}

\begin{equation}
\begin{split}
\frac{1}{3}x_{1} + 2x_{2} = 3 \\
x_{1} + 5x_{2} - 2x_{3} = 2 \\
3x_{3} = 9
\end{split}
\end{equation}

\begin{equation}
\begin{split}
x_{1} + 6x_{2} = 3 \\
x_{1} + 5x_{2} - 2x_{3} = 2 \\
3x_{3} = 9
\end{split}
\end{equation}

\begin{equation}
\begin{split}
x_{1} + 6x_{2} = 9 \\
-x_{2} - 2x_{3} = -7 \\
3x_{3} = 9
\end{split}
\end{equation}

\begin{equation}
\begin{split}
3 + 6 * 1 = 9 \\
-1 - 2 * 3 = -7 \\
3 * 3 = 9
\end{split}
\end{equation}
\end{document}
